wip

theories/cgraph.v
@@ -5,6 +5,8 @@ From stdpp Require Export gmap.
 Require Export diris.multiset.
 From stdpp Require Import fin_maps.
 
+Ltac sdec := repeat case_decide; simplify_eq.
+
 (* Definition uforest V := gset (V * V). *)
 Notation cgraph V L := (gmap V (gmap V L)).
 
@@ -20,7 +22,7 @@ Section cgraph.
     end.
 
   Definition ms_insert (v v' : V) (ev' : gmap V L) (ins : multiset L) : multiset L :=
-    match ev' !! v with | Some l => {[ l ]} ⋅ ins | None => ins end.
+    from_option singleton ε (ev' !! v) ⋅ ins.
 
   Definition in_labels (g : cgraph V L) (v : V) : multiset L :=
     map_fold (ms_insert v) ε g.
@@ -46,26 +48,164 @@ Section cgraph.
     ∀ v1 v2, ¬ (edge g v1 v2 ∧ edge g v2 v1). *)
 
   Section general.
-    Lemma no_self_out_edge g v :
-      cgraph_wf g ->
-      out_edges g v !! v = None.
+
+
+    Lemma in_labels_insert g i x v :
+      g !! i = None ->
+      in_labels (<[i:=x]> g) v ≡ from_option singleton ε (x !! v) ⋅ in_labels g v.
     Proof.
-      intros Hwf.
+      intros Hi.
+      unfold in_labels at 1.
+      erewrite map_fold_insert with (R := (≡));
+      eauto; first apply _; first solve_proper.
+      intros. unfold ms_insert.
+      destruct (z1 !! v) eqn:E;
+      destruct (z2 !! v) eqn:F; simpl; eauto.
+      rewrite assoc.
+      rewrite (comm (⋅) {[ o ]}).
+      rewrite assoc. done.
+    Qed.
+
+    Lemma in_labels_delete g i v y :
+      g !! i = Some y ->
+      from_option singleton ε (y !! v) ⋅ in_labels (delete i g) v ≡ in_labels g v.
+    Proof.
+      intro.
+      pose proof (in_labels_insert (delete i g) i y v) as HH.
+      rewrite insert_delete in HH.
+      rewrite insert_id in HH; eauto.
+      rewrite HH; last by apply lookup_delete.
+      done.
+    Qed.
+
+    Lemma in_labels_update g i x y v :
+      g !! i = Some y ->
+      from_option singleton ε (y !! v) ⋅ in_labels (<[i:=x]> g) v ≡
+      from_option singleton ε (x !! v) ⋅ in_labels g v.
+    Proof.
+      intro.
+      assert (<[i:=x]> g = <[i:=x]> $ delete i g) as -> by by rewrite insert_delete.
+      rewrite in_labels_insert; last by apply lookup_delete.
+      rewrite comm. rewrite -assoc.
+      rewrite (comm (⋅) (in_labels _ _)).
+      rewrite in_labels_delete; eauto.
+    Qed.
+
+    (* Lemma in_labels_dependence g g' v2 :
+      (∀ v1, out_edges g v1 !! v2 = out_edges g' v1 !! v2) ->
+      in_labels g v2 = in_labels g' v2.
+    Proof.
+    Admitted. *)
+
+    Lemma out_edges_in_labels g v1 v2 l :
+      out_edges g v1 !! v2 = Some l ->
+      ∃ x, in_labels g v2 ≡ {[ l ]} ⋅ x.
+    Proof.
+      revert v1 v2 l.
+      induction g using map_ind; intros.
+      - rewrite lookup_empty in H0. simplify_eq.
+      - unfold out_edges in H1. rewrite lookup_insert_spec in H1.
+        case_decide; simplify_eq.
+        + exists (in_labels m v2).
+          rewrite in_labels_insert; eauto.
+          rewrite H1. done.
+        + destruct (m !! v1) eqn:E; simplify_eq.
+          destruct (IHg v1 v2 l).
+          { unfold out_edges. rewrite E. done. }
+          setoid_rewrite in_labels_insert; eauto.
+          setoid_rewrite H3.
+          exists (from_option singleton ε (x !! v2) ⋅ x0).
+          rewrite !assoc.
+          rewrite (comm (⋅) _ {[ l ]}).
+          done.
+    Qed.
+
+    Lemma multiset_empty_mult {A : ofe} (x y : multiset A) :
+      x ⋅ y ≡ ε -> x = ε ∧ y = ε.
+    Proof.
     Admitted.
 
-    Lemma no_self_edge g v1 v2 :
-      cgraph_wf g ->
-      edge g v1 v2 -> v1 ≠ v2.
+    Lemma multiset_empty_neq_singleton {A : ofe} {a : A} :
+      {[ a ]} ≠ ε.
     Proof.
-      intros H1 [] ->.
-      assert (out_edges g v2 !! v2 = None); eauto using no_self_out_edge.
-      rewrite H0 in H2. simplify_eq.
+    Admitted.
+
+    Lemma no_in_labels_no_out_edge g v1 v2 :
+      in_labels g v2 ≡ ε ->
+      out_edges g v1 !! v2 = None.
+    Proof.
+      destruct (out_edges g v1 !! v2) eqn:E; eauto.
+      eapply out_edges_in_labels in E as []. rewrite H0. intros HH.
+      eapply multiset_empty_mult in HH.
+      destruct HH as [H1%multiset_empty_neq_singleton H2]. done.
+    Qed.
+
+    Lemma not_rtsc `{R : A -> A -> Prop} x :
+      (∀ y, ¬ R x y ∧ ¬ R y x) ->
+      (∀ y, rtsc R x y -> x = y).
+    Proof.
+      intros Hy y Hr.
+      induction Hr; eauto. destruct H0; naive_solver.
+    Qed.
+
+    Lemma no_edges_no_uconn g v v' :
+      out_edges g v = ∅ ->
+      in_labels g v ≡ ε ->
+      uconn g v' v -> v = v'.
+    Proof.
+      intros Hout Hin Hconn.
+      eapply not_rtsc; last done.
+      intros y. unfold edge. split; intros [].
+      - rewrite Hout in H0. rewrite lookup_empty in H0. simplify_eq.
+      - eapply no_in_labels_no_out_edge in Hin. erewrite H0 in Hin. simplify_eq.
+    Qed.
+
+    Lemma some_edge (g : cgraph V L) (v1 v2 : V) (l : L) :
+      out_edges g v1 !! v2 = Some l -> edge g v1 v2.
+    Proof.
+      unfold edge. intros ->. eauto.
+    Qed.
+
+
+
+    Lemma not_uconn_out_disjoint g v1 v2 :
+      ¬ uconn g v1 v2 -> out_edges g v1 ##ₘ out_edges g v2.
+    Proof.
+      intros HH v.
+      destruct (out_edges g v1 !! v) eqn:E;
+      destruct (out_edges g v2 !! v) eqn:F; simpl; eauto.
+      assert (edge g v1 v); eauto using some_edge.
+      assert (edge g v2 v); eauto using some_edge.
+      apply HH.
+      eapply rtc_transitive; eapply rtc_once; [left|right]; eauto.
     Qed.
   End general.
 
+  Section empty_cgraph.
+    Lemma out_edges_empty v :
+      out_edges ∅ v = ∅.
+    Proof.
+      unfold out_edges. rewrite lookup_empty //.
+    Qed.
+
+    Lemma in_labels_empty v :
+      in_labels ∅ v ≡ ε.
+    Proof.
+      unfold in_labels. rewrite map_fold_empty. done.
+    Qed.
+
+    Lemma empty_wf :
+      cgraph_wf ∅.
+    Proof.
+    Admitted.
+  End empty_cgraph.
+
   Section insert_edge.
+    (* This function is only supposed to be called if there is not already an edge
+       between v1 and v2. In fact, it's only supposed to be called if v1 and v2
+       are complete disconnected. *)
     Definition insert_edge (g : cgraph V L) (v1 v2 : V) (l : L) :=
-      <[ v1 := out_edges g v1 ∪ {[ v2 := l ]} ]> g.
+      <[ v1 := <[ v2 := l ]> $ out_edges g v1 ]> g.
 
     Lemma out_edges_insert (g : cgraph V L) (v1 v2 : V) e :
       out_edges (<[ v1 := e ]> g) v2 =
@@ -78,7 +218,7 @@ Section cgraph.
 
     Lemma out_edges_insert_edge (g : cgraph V L) (v1 v2 v3 : V) (l : L) :
       out_edges (insert_edge g v1 v2 l) v3 =
-        if decide (v1 = v3) then out_edges g v3 ∪ {[ v2 := l ]}
+        if decide (v1 = v3) then <[ v2 := l ]> $ out_edges g v3
         else out_edges g v3.
     Proof.
       unfold insert_edge. rewrite out_edges_insert.
@@ -91,10 +231,31 @@ Section cgraph.
         if decide (v2 = v3) then {[ l ]} ⋅ in_labels g v3
         else in_labels g v3.
     Proof.
-      unfold insert_edge, in_labels.
-      rewrite map_fold_insert_L.
-      Search map_fold insert.
-    Admitted.
+      intros Hnotedge.
+      unfold insert_edge.
+      destruct (g !! v1) eqn:E.
+      - assert (g !! v1 = Some g0) as HH; eauto.
+        pose proof (in_labels_update g v1 (<[v2:=l]> (out_edges g v1)) g0 v3 HH) as H0.
+        rewrite lookup_insert_spec in H0.
+        destruct (g0 !! v3) eqn:F; simpl in *.
+        + case_decide; simplify_eq; simpl in *.
+          * exfalso. apply Hnotedge.
+            unfold edge. unfold out_edges.
+            rewrite E. rewrite F. eauto.
+          * unfold out_edges in H0 at 2.
+            rewrite E in H0.
+            rewrite F in H0. simpl in *.
+            apply cancelable in H0; eauto; first apply _; done.
+        + rewrite ->left_id in H0. 2: { intro. simpl. rewrite left_id. done. }
+          rewrite H0. case_decide; simpl; eauto. unfold out_edges.
+          rewrite HH. rewrite F. simpl. rewrite left_id. done.
+      - rewrite in_labels_insert; eauto.
+        rewrite lookup_insert_spec.
+        case_decide; simplify_eq; try done.
+        unfold out_edges.
+        rewrite E. rewrite lookup_empty.
+        simpl. rewrite left_id. done.
+    Qed.
 
     Lemma insert_edge_wf g v1 v2 l :
       ¬ uconn g v1 v2 ->
@@ -123,13 +284,51 @@ Section cgraph.
       in_labels g v2 ≡ {[ l ]} ⋅ x ->
       in_labels (delete_edge g v1 v2) v2 ≡ x.
     Proof.
-    Admitted.
+      intros H1 H2.
+      unfold delete_edge.
+      destruct (g !! v1) eqn:E; last first.
+      { unfold out_edges in H1. rewrite E lookup_empty in H1. simplify_eq. }
+      pose proof (in_labels_update g v1 (delete v2 (out_edges g v1)) g0 v2 E) as H0.
+      destruct (g0 !! v2) eqn:F; simpl in *.
+      - rewrite lookup_delete in H0.
+        simpl in *.
+        rewrite ->H2 in H0.
+        unfold out_edges in H1.
+        rewrite E in H1. rewrite F in H1. simplify_eq.
+        revert H0. rewrite left_id. intros H0.
+        apply cancelable in H0; eauto; first apply _; done.
+      - unfold out_edges in H1. rewrite E F in H1. simplify_eq.
+    Qed.
 
     Lemma in_labels_delete_edge_neq (g : cgraph V L) (v1 v2 v3 : V) :
       v2 ≠ v3 ->
       in_labels (delete_edge g v1 v2) v3 ≡ in_labels g v3.
     Proof.
-    Admitted.
+      intros Hneq.
+      unfold delete_edge.
+      destruct (g !! v1) eqn:E.
+      - pose proof (in_labels_update g v1 (delete v2 (out_edges g v1)) g0 v3 E) as H0.
+        destruct (g0 !! v3) eqn:F.
+        + simpl in *.
+          rewrite lookup_delete_spec in H0.
+          unfold out_edges in H0 at 2.
+          rewrite E in H0.
+          rewrite F in H0.
+          case_decide; simplify_eq.
+          simpl in *. apply cancelable in H0; eauto; first apply _; done.
+        + simpl in *. rewrite ->left_id in H0.
+          2: { intro. simpl. rewrite left_id. done. }
+          rewrite H0.
+          rewrite lookup_delete_spec.
+          unfold out_edges. rewrite E.
+          rewrite F. case_decide; simplify_eq; simpl.
+          rewrite left_id. done.
+      - rewrite in_labels_insert; eauto.
+        rewrite lookup_delete_spec.
+        unfold out_edges.
+        rewrite E. rewrite lookup_empty.
+        case_decide; simpl; rewrite left_id //.
+    Qed.
 
     Lemma delete_edge_wf g v1 v2 :
       cgraph_wf g ->
@@ -139,10 +338,94 @@ Section cgraph.
 
     Lemma delete_edge_uconn g v1 v2 :
       cgraph_wf g ->
-      v1 ≠ v2 ->
+      edge g v1 v2 ->
       ¬ uconn (delete_edge g v1 v2) v1 v2.
     Proof.
     Admitted.
+
+    Lemma edge_delete_edge g v1 v2 w1 w2 :
+      v1 ≠ w1 ∨ v2 ≠ w2 ->
+      edge g w1 w2 ->
+      edge (delete_edge g v1 v2) w1 w2.
+    Proof.
+      intros.
+      unfold edge.
+      rewrite out_edges_delete_edge.
+      case_decide; simplify_eq; eauto.
+      rewrite lookup_delete_spec.
+      case_decide; simplify_eq; eauto.
+      naive_solver.
+    Qed.
+
+    Lemma edge_delete_edge' g v1 v2 w1 w2 :
+      edge g w1 w2 ->
+      edge (delete_edge g v1 v2) w1 w2 ∨ (v1 = w1 ∧ v2 = w2).
+    Proof.
+      intros.
+      pose proof (edge_delete_edge g v1 v2 w1 w2).
+      destruct (decide (v1 = w1));
+      destruct (decide (v2 = w2));
+      naive_solver.
+    Qed.
+
+    Lemma no_self_edge g v1 v2 :
+      cgraph_wf g ->
+      edge g v1 v2 -> v1 ≠ v2.
+    Proof.
+      intros H1 H2 ->.
+      eapply delete_edge_uconn; eauto. reflexivity.
+    Qed.
+
+    Lemma no_self_edge' g v1 v2 :
+      cgraph_wf g ->
+      sc (edge g) v1 v2 -> v1 ≠ v2.
+    Proof.
+      intros H1 [] ->; eapply no_self_edge; eauto.
+    Qed.
+
+    Lemma no_self_edge'' g v :
+      cgraph_wf g ->
+      out_edges g v !! v = None.
+    Proof.
+      intros.
+      destruct (_!!_) eqn:E; eauto.
+      exfalso.
+      eapply no_self_edge; eauto using some_edge.
+    Qed.
+
+    Lemma no_triangle g v1 v2 v3 :
+      cgraph_wf g ->
+      sc (edge g) v1 v2 ->
+      sc (edge g) v2 v3 ->
+      sc (edge g) v3 v1 ->
+      False.
+    Proof.
+      intros Hwf H1 H2 H3.
+      assert (v1 ≠ v2); eauto using no_self_edge'.
+      assert (v2 ≠ v3); eauto using no_self_edge'.
+      assert (v3 ≠ v1); eauto using no_self_edge'.
+      destruct H1,H2,H3; eapply delete_edge_uconn; eauto;
+      eapply rtc_transitive; eapply rtc_once;
+      try (solve [left; eapply edge_delete_edge; eauto] ||
+           solve [right; eapply edge_delete_edge; eauto]).
+      - left. eapply edge_delete_edge; eauto.
+      - left. eapply edge_delete_edge.
+        + right. intro. eapply H4. symmetry. done.
+        + eauto.
+      - right. eapply edge_delete_edge; eauto.
+    Qed.
+
+    Lemma edge_out_disjoint g v1 v2 :
+      cgraph_wf g -> edge g v1 v2 -> out_edges g v1 ##ₘ out_edges g v2.
+    Proof.
+      intros Hwf Hv12 v.
+      destruct (out_edges g v1 !! v) eqn:E;
+      destruct (out_edges g v2 !! v) eqn:F; simpl; eauto.
+      eapply no_triangle; eauto.
+      - left. eauto.
+      - left. unfold edge. erewrite F. eauto.
+      - right. unfold edge. rewrite E. eauto.
+    Qed.
   End delete_edge.
 
 
@@ -160,13 +443,7 @@ Section cgraph.
       rewrite out_edges_delete_edge.
       repeat case_decide; simplify_eq; eauto.
       apply map_eq. intros v.
-      rewrite lookup_insert_spec.
-      rewrite lookup_union.
-      rewrite lookup_delete_spec.
-      repeat case_decide; simplify_eq.
-      + rewrite lookup_singleton. simpl. done.
-      + rewrite lookup_singleton_ne; eauto.
-        destruct (_ !! _); done.
+      rewrite insert_delete //.
     Qed.
 
     Lemma update_in_labels_eq g v1 v2 l l' x :
@@ -202,7 +479,6 @@ Section cgraph.
       unfold update_edge.
       apply insert_edge_wf.
       - apply delete_edge_uconn; eauto.
-        eapply no_self_edge; eauto.
       - eapply delete_edge_wf; eauto.
     Qed.
   End update_edge.
@@ -216,231 +492,449 @@ Section cgraph.
       | None => g
       end.
 
-    Lemma move_edge_out_edges g v1 v2 v3 v :
-      out_edges (move_edge g v1 v2 v3) v = ∅.
+    Lemma move_edge_out_edges g v1 v2 v3 v l :
+      out_edges g v1 !! v3 = Some l ->
+      out_edges (move_edge g v1 v2 v3) v =
+        if decide (v = v2) then <[ v3 := l ]> $ out_edges g v
+        else if decide (v = v1) then delete v3 $ out_edges g v
+        else out_edges g v.
     Proof.
-    Admitted.
+      intros H1.
+      unfold move_edge. rewrite H1.
+      rewrite out_edges_insert_edge.
+      rewrite out_edges_delete_edge.
+      repeat case_decide; simplify_eq; eauto; apply map_eq; intro;
+      rewrite ?lookup_union ?lookup_insert_spec ?lookup_delete_spec ?lookup_empty;
+      repeat case_decide; simplify_eq; eauto.
+    Qed.
 
-    
+    Lemma move_edge_in_labels g v1 v2 v3 v :
+      cgraph_wf g ->
+      sc (edge g) v1 v2 ->
+      in_labels (move_edge g v1 v2 v3) v ≡ in_labels g v.
+    Proof.
+      intros Hwf Hv12.
+      unfold move_edge.
+      destruct (_!!_) eqn:E; eauto.
+      rewrite in_labels_insert_edge.
+      - case_decide; simplify_eq.
+        + destruct (out_edges_in_labels _ _ _ _ E).
+          rewrite in_labels_delete_edge_eq; eauto.
+          by symmetry.
+        + rewrite in_labels_delete_edge_neq; eauto.
+      - unfold edge.
+        assert (v1 ≠ v2); eauto using no_self_edge'.
+        rewrite out_edges_delete_edge.
+        case_decide; simplify_eq.
+        intro HH.
+        eapply no_triangle; eauto.
+        + left; eauto.
+        + right. unfold edge. erewrite E. eauto.
+    Qed.
+
+    Lemma move_edge_in_labels' g v1 v2 v3 v :
+      cgraph_wf g ->
+      ¬ uconn g v1 v2 ->
+      in_labels (move_edge g v1 v2 v3) v ≡ in_labels g v.
+    Proof.
+      intros Hwf Hv12.
+      unfold move_edge.
+      destruct (_!!_) eqn:E; eauto.
+      rewrite in_labels_insert_edge.
+      - case_decide; simplify_eq.
+        + destruct (out_edges_in_labels _ _ _ _ E).
+          rewrite in_labels_delete_edge_eq; eauto.
+          by symmetry.
+        + rewrite in_labels_delete_edge_neq; eauto.
+      - unfold edge.
+        assert (v1 ≠ v2). { intros ->. apply Hv12. reflexivity. }
+        rewrite out_edges_delete_edge.
+        case_decide; simplify_eq.
+        intros [].
+        assert (edge g v1 v3); eauto using some_edge.
+        assert (edge g v2 v3); eauto using some_edge.
+        apply Hv12.
+        eapply rtc_transitive; eapply rtc_once;[left|right]; eauto.
+    Qed.
+
+    Lemma move_edge_wf g v1 v2 v3 :
+      v2 ≠ v3 ->
+      cgraph_wf g ->
+      sc (edge g) v1 v2 ->
+      cgraph_wf (move_edge g v1 v2 v3).
+    Proof.
+      intros Hneq Hwf Hv12.
+      unfold move_edge.
+      destruct (_!!_) eqn:E; eauto.
+      apply insert_edge_wf; eauto using delete_edge_wf.
+      intro Hconn.
+      eapply (delete_edge_uconn g v1 v3); eauto.
+      - unfold edge. rewrite E. eauto.
+      - unfold uconn in *.
+        assert (sc (edge (delete_edge g v1 v3)) v1 v2). {
+          destruct Hv12.
+          - left. unfold edge. rewrite out_edges_delete_edge.
+            case_decide; simplify_eq.
+            rewrite lookup_delete_ne; eauto.
+          - right. unfold edge. rewrite out_edges_delete_edge.
+            case_decide; simplify_eq; eauto.
+            exfalso. eapply no_self_edge; eauto.
+        }
+        eapply transitivity; last done.
+        econstructor; first done.
+        econstructor.
+    Qed.
+
+    Lemma edge_delete_edge'' g v1 v2 w1 w2 :
+      edge (delete_edge g w1 w2) v1 v2 -> edge g v1 v2.
+    Proof.
+      rewrite /delete_edge /edge /out_edges.
+      destruct (g !! w1) eqn:F; simpl; rewrite lookup_insert_spec; repeat case_decide;
+      rewrite ?lookup_delete_spec; repeat case_decide; simplify_eq;
+      try destruct (g !! v1) eqn:E; simpl; rewrite ?lookup_empty; eauto; try intros [];
+      simplify_eq. rewrite H0. eauto.
+    Qed.
+
+    Lemma delete_edge_preserves_not_uconn g v1 v2 w1 w2 :
+      uconn (delete_edge g w1 w2) v1 v2 -> uconn g v1 v2.
+    Proof.
+      intros HH. induction HH; try reflexivity.
+      eapply rtc_transitive; eauto. eapply rtc_once.
+      destruct H0; [left|right]; eauto using edge_delete_edge''.
+    Qed.
+
+    Lemma move_edge_wf' g v1 v2 v3 :
+      v2 ≠ v3 ->
+      cgraph_wf g ->
+      ¬ uconn g v1 v2 ->
+      cgraph_wf (move_edge g v1 v2 v3).
+    Proof.
+      intros Hneq Hwf Hv12.
+      unfold move_edge.
+      destruct (_!!_) eqn:E; eauto.
+      apply insert_edge_wf; eauto using delete_edge_wf.
+      assert (¬ uconn g v3 v2).
+      { intro. apply Hv12.
+        eapply rtc_transitive; eauto.
+        eapply rtc_once. left. eauto using some_edge. }
+      intro. apply delete_edge_preserves_not_uconn in H1.
+      apply H0. symmetry. done.
+    Qed.
+
+    Definition cgraph_equiv g1 g2 :=
+      ∀ v, out_edges g1 v = out_edges g2 v.
+
+    Lemma cgraph_equiv_edge g1 g2 v1 v2 :
+      cgraph_equiv g1 g2 ->
+      edge g1 v1 v2 ->
+      edge g2 v1 v2.
+    Proof.
+      unfold edge. intros ->. done.
+    Qed.
+
+    Lemma uconn_equiv g1 g2 v1 v2 :
+      cgraph_equiv g1 g2 ->
+      uconn g1 v1 v2 -> uconn g2 v1 v2.
+    Proof.
+      intros He Hc.
+      induction Hc; try reflexivity.
+      eapply rtc_transitive; eauto.
+      eapply rtc_once.
+      destruct H0;[left|right]; eauto using cgraph_equiv_edge.
+    Qed.
+
+    Lemma move_edge_uconn g v1 v2 v3 :
+      cgraph_wf g ->
+      ¬ uconn g v1 v2 ->
+      ¬ uconn (move_edge g v1 v2 v3) v1 v2.
+    Proof.
+      intros Hwf H1.
+      destruct (out_edges g v1 !! v3) eqn:E; last first.
+      { unfold move_edge. rewrite E. done. }
+      assert (¬ uconn (delete_edge (move_edge (insert_edge g v1 v2 o) v1 v2 v3) v1 v2) v1 v2).
+      {
+        eapply delete_edge_uconn.
+        - eapply move_edge_wf.
+          + intros ->. eapply H1. eapply rtc_once. left. eauto using some_edge.
+          + eapply insert_edge_wf; eauto.
+          + left. unfold edge.
+            rewrite out_edges_insert_edge.
+            case_decide; simplify_eq. rewrite lookup_insert. eauto.
+        - unfold edge.
+          erewrite move_edge_out_edges; last first.
+          + rewrite out_edges_insert_edge.
+            case_decide; simplify_eq.
+            rewrite lookup_insert_spec.
+            case_decide; simplify_eq; eauto.
+          + rewrite !out_edges_insert_edge.
+            repeat case_decide; simplify_eq.
+            * rewrite !lookup_insert_spec.
+              case_decide; simplify_eq. eauto.
+            * rewrite lookup_delete_spec lookup_insert_spec.
+              case_decide; simplify_eq.
+              -- exfalso. apply H1.
+                 eapply rtc_once. left. eauto using some_edge.
+              -- case_decide; simplify_eq. eauto.
+      }
+      intro. apply H0.
+      eapply uconn_equiv; eauto.
+      intro.
+      rewrite out_edges_delete_edge.
+      erewrite move_edge_out_edges; last done.
+      erewrite move_edge_out_edges; last first.
+      { rewrite out_edges_insert_edge. case_decide; eauto.
+        rewrite lookup_insert_spec. case_decide; simplify_eq; eauto. }
+      rewrite !out_edges_insert_edge.
+      repeat case_decide; simplify_eq; eauto.
+      - assert (v2 ≠ v3). { intros ->. eapply no_self_edge; eauto using some_edge. }
+        rewrite delete_insert_ne; eauto.
+        rewrite delete_insert; eauto.
+        destruct (out_edges g v2 !! v2) eqn:F; eauto.
+        exfalso. eapply no_self_edge; eauto using some_edge.
+      - rewrite delete_commute.
+        rewrite delete_insert; eauto.
+        destruct (out_edges g v !! v2) eqn:F; eauto.
+        exfalso. apply H1. apply rtc_once.
+        left. eapply some_edge; eauto.
+    Qed.
   End move_edge.
 
+  Section move_edges.
+    Lemma move_edges g v1 v2 e1 e2 :
+      cgraph_wf g ->
+      ¬ uconn g v1 v2 ->
+      e1 ##ₘ e2 ->
+      out_edges g v1 = e1 ∪ e2 ->
+      ∃ g', cgraph_wf g' ∧
+        ¬ uconn g' v1 v2 ∧
+        (∀ v, out_edges g' v =
+          if decide (v = v1) then e1
+          else if decide (v = v2) then out_edges g v ∪ e2
+          else out_edges g v) ∧
+        (∀ v, in_labels g' v ≡ in_labels g v).
+    Proof.
+      revert g e1.
+      induction e2 using map_ind; intros g e1;
+      intros Hwf Hnuconn Hdisj Hout.
+      - exists g. rewrite right_id_L in Hout.
+        split_and!; eauto. intro.
+        repeat case_decide; simplify_eq; eauto.
+        rewrite right_id_L //.
+      - specialize (IHe2 (move_edge g v1 v2 i) e1).
+        destruct IHe2.
+        + apply move_edge_wf'; eauto. intros ->. apply Hnuconn.
+          apply rtc_once.
+          left.
+          unfold edge.
+          rewrite Hout.
+          rewrite lookup_union lookup_insert.
+          destruct (e1 !! i); eauto.
+        + apply move_edge_uconn; eauto.
+        + solve_map_disjoint.
+        + destruct (out_edges g v1 !! i) eqn:E.
+          2: { rewrite Hout in E. rewrite lookup_union lookup_insert in E.
+            destruct (e1 !! i); simpl in *; simplify_eq.  }
+          erewrite move_edge_out_edges; eauto.
+          repeat case_decide; simplify_eq.
+          -- exfalso. apply Hnuconn. reflexivity.
+          -- rewrite Hout. rewrite delete_union.
+             rewrite delete_insert; eauto.
+             rewrite delete_notin; eauto.
+             solve_map_disjoint.
+        + destruct H1 as (H1 & H2 & H3 & H4).
+          exists x0. split_and!; eauto.
+          -- intros v. rewrite H3.
+             assert (out_edges g v1 !! i = Some x).
+             { rewrite Hout. rewrite lookup_union lookup_insert.
+                destruct (e1 !! i) eqn:E; simpl; eauto.
+                specialize (Hdisj i). rewrite E in Hdisj. rewrite lookup_insert in Hdisj.
+                simpl in *. done. }
+             repeat case_decide; simplify_eq; eauto.
+             ++ erewrite move_edge_out_edges; eauto.
+                case_decide; simplify_eq.
+                apply map_eq; intro.
+                rewrite !lookup_union !lookup_insert_spec;
+                repeat case_decide; simplify_eq; eauto.
+                rewrite H0. simpl.
+                destruct (out_edges g v2 !! i0) eqn:E; eauto; simpl.
+                exfalso.
+                apply Hnuconn.
+                eapply rtc_transitive; eapply rtc_once; [left|right];
+                eauto using some_edge.
+             ++ erewrite move_edge_out_edges; eauto.
+                repeat case_decide; simplify_eq. done.
+          -- intros v. rewrite H4. rewrite move_edge_in_labels'; eauto.
+    Qed.
+
+    Lemma move_edges' g v1 v2 e1 e2 :
+      cgraph_wf g ->
+      ¬ uconn g v1 v2 ->
+      e1 ##ₘ e2 ->
+      out_edges g v1 = e1 ∪ e2 ->
+      ∃ g', cgraph_wf g' ∧
+        ¬ uconn g' v1 v2 ∧
+        out_edges g' v1 = e1 ∧
+        out_edges g' v2 = out_edges g v2 ∪ e2 ∧
+        (∀ v, v ≠ v1 -> v ≠ v2 -> out_edges g' v = out_edges g v) ∧
+        (∀ v, in_labels g' v ≡ in_labels g v).
+    Proof.
+      intros.
+      edestruct move_edges as (?&?&?&?&?); eauto.
+      eexists. split_and!; eauto.
+      - specialize (H6 v1). case_decide; simplify_eq; done.
+      - specialize (H6 v2). repeat case_decide; simplify_eq; done.
+      - intros. specialize (H6 v); repeat case_decide; simplify_eq; eauto.
+    Qed.
+  End move_edges.
 
 
+  Lemma gmap_xsplit (e1 e2 e1' e2' : gmap V L) :
+    e1 ##ₘ e2 ->
+    e1' ##ₘ e2' ->
+    e1 ∪ e2 = e1' ∪ e2' ->
+    ∃ e11 e12 e21 e22,
+      e11 ##ₘ e12 ∧ e21 ##ₘ e22 ∧
+      e11 ##ₘ e21 ∧ e12 ##ₘ e22 ∧
+      e1 = e11 ∪ e12 ∧ e2 = e21 ∪ e22 ∧
+      e1' = e11 ∪ e21 ∧ e2' = e12 ∪ e22.
+  Proof. Admitted.
+    
+
+  Section exchange.
+    Lemma exchange g v1 v2 e1 e2 :
+      cgraph_wf g ->
+      ¬ uconn g v1 v2 ->
+      e1 ##ₘ e2 ->
+      out_edges g v1 ∪ out_edges g v2 = e1 ∪ e2 ->
+      ∃ g', cgraph_wf g' ∧
+        ¬ uconn g' v1 v2 ∧
+        out_edges g' v1 = e1 ∧
+        out_edges g' v2 = e2 ∧
+        (∀ v, v ≠ v1 -> v ≠ v2 -> out_edges g' v = out_edges g v) ∧
+        (∀ v, in_labels g' v ≡ in_labels g v).
+    Proof.
+      intros Hwf Hnuconn Hdisj Hsplit.
+      assert (out_edges g v1 ##ₘ out_edges g v2) as Hdisj'.
+      { apply not_uconn_out_disjoint. done. }
+      destruct (gmap_xsplit _ _ _ _ Hdisj' Hdisj Hsplit)
+        as (e11 & e12 & e21 & e22 & Hdisj1 & Hdisj2 & Hdisj3 & Hdisj4 &
+            ? & ? & HH1 & HH2); subst.
+
+      destruct (move_edges' g v1 v2 e11 e12)
+        as (g' & Hwf' & Hnuconn' & Hv1 & Hv2 & Hv & Hin); eauto.
+      rewrite H1 in Hv2.
+      rewrite <-assoc in Hv2; last apply _.
+      rewrite map_union_comm in Hv2; last solve_map_disjoint.
+
+      destruct (move_edges' g' v2 v1 (e22 ∪ e12) e21)
+        as (g'' & Hwf'' & Hnuconn'' & Hv1' & Hv2' & Hv' & Hin'); eauto.
+      { intro. apply Hnuconn'. symmetry. done. }
+      { solve_map_disjoint. }
+
+      eexists. split_and!; eauto.
+      - intro. symmetry in H2. eauto.
+      - rewrite Hv2' Hv1 //.
+      - rewrite Hv1'. rewrite map_union_comm; eauto.
+      - intros. rewrite Hv'; eauto.
+      - intros. rewrite Hin'. eauto.
+    Qed.
+  End exchange.
+
+  Section exchange_alloc.
+    Lemma exchange_alloc g v1 v2 e1 e2 l :
+      cgraph_wf g ->
+      ¬ uconn g v1 v2 ->
+      e1 ##ₘ e2 ->
+      out_edges g v1 ∪ out_edges g v2 = e1 ∪ e2 ->
+      ∃ g', cgraph_wf g' ∧
+        out_edges g' v1 = <[v2:=l]> e1 ∧
+        out_edges g' v2 = e2 ∧
+        (∀ v, v ≠ v1 -> v ≠ v2 -> out_edges g' v = out_edges g v) ∧
+        in_labels g' v2 ≡ {[ l ]} ⋅ in_labels g v2 ∧
+        (∀ v, v ≠ v2 -> in_labels g' v ≡ in_labels g v).
+    Proof.
+      intros Hwf Hnuconn Hdisj Hsplit.
+      destruct (exchange g v1 v2 e1 e2)
+        as (g' & Hwf' & Hnuconn' & Hout1 & Hout2 & Hrest & Hin); eauto.
+      exists (insert_edge g' v1 v2 l).
+      split_and!.
+      - eapply insert_edge_wf; eauto.
+      - rewrite out_edges_insert_edge. sdec; done.
+      - rewrite out_edges_insert_edge. sdec; eauto.
+        exfalso. apply Hnuconn'. reflexivity.
+      - intros. rewrite out_edges_insert_edge. sdec. eauto.
+      - rewrite in_labels_insert_edge.
+        + sdec. rewrite Hin. done.
+        + intro. eapply Hnuconn'. eapply rtc_once. left. done.
+      - intros. rewrite in_labels_insert_edge.
+        + sdec. rewrite Hin. done.
+        + intro. eapply Hnuconn'. eapply rtc_once. left. done.
+    Qed.
+  End exchange_alloc.
 
 
+  Section exchange_dealloc.
+    Lemma exchange_dealloc g v1 v2 e1 e2 l :
+      cgraph_wf g ->
+      out_edges g v1 !! v2 = Some l ->
+      e1 ##ₘ e2 ->
+      delete v2 (out_edges g v1) ∪ out_edges g v2 = e1 ∪ e2 ->
+      ∃ g', cgraph_wf g' ∧
+        ¬ uconn g' v1 v2 ∧
+        out_edges g' v1 = e1 ∧
+        out_edges g' v2 = e2 ∧
+        (∀ v, v ≠ v1 -> v ≠ v2 -> out_edges g' v = out_edges g v) ∧
+        (∀ x, in_labels g v2 ≡ {[ l ]} ⋅ x -> in_labels g' v2 ≡ x) ∧
+        (∀ v, v ≠ v2 -> in_labels g' v ≡ in_labels g v).
+    Proof.
+      intros Hwf H1 Hdisj Hsplit.
+      destruct (exchange (delete_edge g v1 v2) v1 v2 e1 e2)
+        as (g' & Hwf' & Hnuconn' & Hout1 & Hout2 & Hrest & Hin).
+      - eapply delete_edge_wf; eauto.
+      - eapply delete_edge_uconn; eauto using some_edge.
+      - eauto.
+      - rewrite !out_edges_delete_edge. sdec; eauto.
+        exfalso. eapply no_self_edge; eauto using some_edge.
+      - exists g'. split_and!; eauto.
+        + intros. rewrite Hrest; eauto.
+          rewrite out_edges_delete_edge. sdec. done.
+        + intros. rewrite Hin. rewrite in_labels_delete_edge_eq; last done; eauto.
+        + intros. rewrite Hin.
+          rewrite in_labels_delete_edge_neq; eauto.
+    Qed.
+  End exchange_dealloc.
 
-
-
-  Lemma cgraph_wellfounded (R : V -> V -> Prop) g :
-  (* Problem: self loops *)
-    cgraph_wf g ->
-    antisymmetric V R ->
-    (∀ x y, R x y -> sc (edge g) x y) ->
-    wf R.
-  Proof.
-  Admitted.
-
-  Lemma not_rtsc `{R : A -> A -> Prop} x :
-    (∀ y, ¬ R x y ∧ ¬ R y x) ->
-    (∀ y, rtsc R x y -> x = y).
-  Proof.
-    Search rtsc.
-  Admitted.
-
-  Lemma multiset_empty_mult {A : ofe} (x y : multiset A) :
-    x ⋅ y ≡ ε -> x = ε ∧ y = ε.
-  Proof.
-  Admitted.
-
-  Lemma multiset_empty_neq_singleton {A : ofe} {a : A} :
-    {[ a ]} ≠ ε.
-  Proof.
-  Admitted.
-
-  Lemma out_edges_in_labels g v1 v2 l :
-    out_edges g v1 !! v2 = Some l ->
-    ∃ x, in_labels g v2 ≡ {[ l ]} ⋅ x.
-  Proof.
-  Admitted.
-
-  Lemma no_in_labels_no_out_edge g v1 v2 :
-    in_labels g v2 ≡ ε ->
-    out_edges g v1 !! v2 = None.
-  Proof.
-    destruct (out_edges g v1 !! v2) eqn:E; eauto.
-    eapply out_edges_in_labels in E as []. rewrite H0. intros HH.
-    eapply multiset_empty_mult in HH.
-    destruct HH as [H1%multiset_empty_neq_singleton H2]. done.
-  Qed.
-
-  Lemma no_edges_no_uconn g v v' :
-    out_edges g v = ∅ ->
-    in_labels g v ≡ ε ->
-    uconn g v' v -> v = v'.
-  Proof.
-    intros Hout Hin Hconn.
-    eapply not_rtsc; last done.
-    intros y. unfold edge. split; intros [].
-    - rewrite Hout in H0. rewrite lookup_empty in H0. simplify_eq.
-    - eapply no_in_labels_no_out_edge in Hin. erewrite H0 in Hin. simplify_eq.
-  Qed.
-
-  Lemma some_edge (g : cgraph V L) (v1 v2 : V) (l : L) :
-    out_edges g v1 !! v2 = Some l -> edge g v1 v2.
-  Proof.
-    unfold edge. intros ->. eauto.
-  Qed.
-
-  Lemma edge_out_disjoint g v1 v2 :
-    cgraph_wf g -> edge g v1 v2 -> out_edges g v1 ##ₘ out_edges g v2.
-  Proof.
-  Admitted.
-
-  Lemma no_self_out_edge g v :
-    cgraph_wf g ->
-    out_edges g v !! v = None.
-  Proof.
-    intros Hwf.
-    pose proof (cgraph_wellfounded (λ x y, x = v ∧ y = v) g Hwf).
-  Admitted.
-
-  Lemma out_edges_empty v :
-    out_edges ∅ v = ∅.
-  Proof.
-    unfold out_edges. rewrite lookup_empty //.
-  Qed.
-
-  Lemma in_labels_empty v :
-    in_labels ∅ v ≡ ε.
-  Proof.
-    unfold in_labels. rewrite map_fold_empty. done.
-  Qed.
-
-  Lemma empty_wf :
-    cgraph_wf ∅.
-  Proof.
-    split.
-    - intros ??[[] []].
-      rewrite out_edges_empty in H0.
-      rewrite lookup_empty in H0.
-      simplify_eq.
-    - admit.
-  Admitted.
-
-
-
-
-  Lemma delete_edge_uconn g v1 v2 :
-    edge g v1 v2 ->
-    cgraph_wf g ->
-    ¬ uconn (delete_edge g v1 v2) v1 v2.
-  Proof.
-  Admitted.
-
-  Definition exchange (g : cgraph V L) v1 v2 l' e1 e2 :=
-    <[ v1 := e1 ∪ {[ v2 := l' ]} ]> $ <[ v2 := e2 ]> g.
-
-  Definition exchange_valid g v1 v2 e1 e2 :=
-    edge g v1 v2 ∧ e1 ##ₘ e2 ∧ e1 ∪ e2 = (delete v2 $ out_edges g v1) ∪ out_edges g v2.
-
-  Lemma exchange_wf g v1 v2 l' e1 e2 :
-    exchange_valid g v1 v2 e1 e2 ->
-    cgraph_wf g ->
-    cgraph_wf (exchange g v1 v2 l' e1 e2).
-  Proof.
-  Admitted.
-
-  Lemma exchange_in_labels g v1 v2 v3 l l' e1 e2 x :
-    exchange_valid g v1 v2 e1 e2 ->
-    in_labels g v2 ≡ {[ l ]} ⋅ x ->
-    cgraph_wf g ->
-    in_labels (exchange g v1 v2 l' e1 e2) v3 =
-      if decide (v3 = v2) then {[ l' ]} ⋅ x
-      else in_labels g v3.
-  Proof.
-  Admitted.
-
-  Lemma exchange_out_edges g v1 v2 v3 l' e1 e2 :
-    out_edges (exchange g v1 v2 l' e1 e2) v3 =
-      if decide (v3 = v1) then e1 ∪ {[ v2 := l' ]}
-      else if decide (v3 = v2) then e2
-      else out_edges g v3.
-  Proof.
-    unfold exchange.
-    unfold out_edges.
-    rewrite !lookup_insert_spec.
-    repeat case_decide; simplify_eq; eauto.
-  Qed.
-
-  Definition dealloc (g : cgraph V L) v1 v2 e1 e2 :=
-    <[ v1 := e1 ]> $ <[ v2 := e2 ]> g.
-
-  Definition dealloc_valid g v1 v2 e1 e2 :=
-    edge g v1 v2 ∧ e1 ##ₘ e2 ∧ e1 ∪ e2 = (delete v2 $ out_edges g v1) ∪ out_edges g v2.
-
-
-  Lemma dealloc_wf g v1 v2 e1 e2 :
-    dealloc_valid g v1 v2 e1 e2 ->
-    cgraph_wf g ->
-    cgraph_wf (dealloc g v1 v2 e1 e2).
-  Proof.
-  Admitted.
-
-  Lemma dealloc_in_labels g v1 v2 v3 l e1 e2 x :
-    dealloc_valid g v1 v2 e1 e2 ->
-    in_labels g v2 ≡ {[ l ]} ⋅ x ->
-    cgraph_wf g ->
-    in_labels (dealloc g v1 v2 e1 e2) v3 =
-      if decide (v3 = v2) then x
-      else in_labels g v3.
-  Proof.
-  Admitted.
-
-  Lemma dealloc_out_edges g v1 v2 v3 e1 e2 :
-    out_edges (dealloc g v1 v2 e1 e2) v3 =
-      if decide (v3 = v1) then e1
-      else if decide (v3 = v2) then e2
-      else out_edges g v3.
-  Proof.
-    unfold dealloc.
-    unfold out_edges.
-    rewrite !lookup_insert_spec.
-    repeat case_decide; simplify_eq; eauto.
-  Qed.
-
-  Definition alloc (g : cgraph V L) v1 v2 l' e1 e2 :=
-    <[ v1 := e1 ∪ {[ v2 := l' ]} ]> $ <[ v2 := e2 ]> g.
-
-  Definition alloc_valid g v1 v2 e1 e2 :=
-    ¬ (uconn g v1 v2) ∧ e1 ##ₘ e2 ∧ e1 ∪ e2 = out_edges g v1 ∪ out_edges g v2.
-
-  Lemma alloc_wf g v1 v2 l' e1 e2 :
-    alloc_valid g v1 v2 e1 e2 ->
-    cgraph_wf g ->
-    cgraph_wf (alloc g v1 v2 l' e1 e2).
-  Proof.
-  Admitted.
-
-  Lemma alloc_in_labels g v1 v2 v3 l' e1 e2 :
-    alloc_valid g v1 v2 e1 e2 ->
-    cgraph_wf g ->
-    in_labels (alloc g v1 v2 l' e1 e2) v3 =
-      if decide (v3 = v2) then {[ l' ]} ⋅ in_labels g v2
-      else in_labels g v3.
-  Proof.
-  Admitted.
-
-  Lemma alloc_out_edges g v1 v2 v3 l' e1 e2 :
-    out_edges (alloc g v1 v2 l' e1 e2) v3 =
-      if decide (v3 = v1) then e1 ∪ {[ v2 := l' ]}
-      else if decide (v3 = v2) then e2
-      else out_edges g v3.
-  Proof.
-    unfold alloc.
-    unfold out_edges.
-    rewrite !lookup_insert_spec.
-    repeat case_decide; simplify_eq; eauto.
-  Qed.
-
+  Section exchange_relabel.
+    Lemma exchange_relabel g v1 v2 e1 e2 l l' :
+      cgraph_wf g ->
+      out_edges g v1 !! v2 = Some l ->
+      e1 ##ₘ e2 ->
+      delete v2 (out_edges g v1) ∪ out_edges g v2 = e1 ∪ e2 ->
+      ∃ g', cgraph_wf g' ∧
+        out_edges g' v1 = <[v2:=l']> e1 ∧
+        out_edges g' v2 = e2 ∧
+        (∀ v, v ≠ v1 -> v ≠ v2 -> out_edges g' v = out_edges g v) ∧
+        (∀ x, in_labels g v2 ≡ {[ l ]} ⋅ x -> in_labels g' v2 ≡ {[ l' ]} ⋅ x) ∧
+        (∀ v, v ≠ v2 -> in_labels g' v ≡ in_labels g v).
+    Proof.
+      intros Hwf H1 Hdisj Hsplit.
+      destruct (exchange_dealloc g v1 v2 e1 e2 l)
+        as (g' & Hwf' & Hnuconn' & Hout1 & Hout2 & Hrest & Hin2 & Hin); eauto.
+      exists (insert_edge g' v1 v2 l').
+      split_and!; eauto.
+      - eapply insert_edge_wf; eauto.
+      - rewrite out_edges_insert_edge. sdec; done.
+      - rewrite out_edges_insert_edge. sdec; eauto.
+        exfalso. apply Hnuconn'. reflexivity.
+      - intros. rewrite out_edges_insert_edge. sdec.
+        rewrite Hrest; eauto.
+      - intros. rewrite in_labels_insert_edge.
+        + sdec. rewrite Hin2; done.
+        + intro. eapply Hnuconn'. eapply rtc_once. left. done.
+      - intros. rewrite in_labels_insert_edge.
+        + sdec. rewrite Hin; done.
+        + intro. eapply Hnuconn'. eapply rtc_once. left. done.
+    Qed.
+  End exchange_relabel.
 
 End cgraph.
