theories/todo.md
@@ -1,4 +1,20 @@
 * (? of ?) prove connectivity graph lemmas
+  - Prove in_labels lemmas [done]
+  - Refactor exchange, alloc, and dealloc to use lemmas+existentials [done]
+  - Do move_multi [done]
+  - Do move_bidir [done]
+  - Prove the exchange, alloc, and dealloc lemmas [done]
+  - Update genericinv.v to use those new lemmas
+    + inv_exchange [done]
+    + inv_dealloc
+    + inv_alloc_l
+    + inv_alloc_r
+    + update invariant2.v
+  - Define cgraph_wf
+  - Prove insert_edge_wf and delete_edge_wf and empty_wf
+  - State adequacy lemma for cgraphs
+  - Prove adequacy lemma for cgraphs
+  - Prove no_triangle
 * (5 of 5) state the generic invariant lemmas
 * (5 of 5) prove the generic invariant lemmas
 * (5 of 5) prove preservation using generic invariant library
